src/lowparse/LowParse.SLow.DER.fst
@@ -1,0 +1,57 @@
+module LowParse.SLow.DER
+include LowParse.Spec.DER
+include LowParse.SLow.Combinators
+include LowParse.SLow.VLData // for bounded_integer
+open FStar.Mul
+
+module Seq = FStar.Seq
+module U8 = FStar.UInt8
+module E = LowParse.BigEndian
+module U32 = FStar.UInt32
+module Math = LowParse.Math
+
+#reset-options "--z3cliopt smt.arith.nl=false --max_fuel 0 --max_ifuel 0"
+
+let be_int_of_bounded_integer
+  (len: integer_size)
+  (x: nat { x < pow2 (8 * len) } )
+: GTot (bounded_integer len)
+= integer_size_values len;
+  assert_norm (pow2 (8 * 1) == 256);
+  assert_norm (pow2 (8 * 2) == 65536);
+  assert_norm (pow2 (8 * 3) == 16777216);
+  assert_norm (pow2 (8 * 4) == 4294967296);
+  U32.uint_to_t x
+
+let be_int_of_bounded_integer_injective
+  (len: integer_size)
+: Lemma
+  (synth_injective (be_int_of_bounded_integer len))
+  [SMTPat (synth_injective (be_int_of_bounded_integer len))] // FIXME: WHY WHY WHY does this pattern NEVER trigger?
+= integer_size_values len;
+  assert_norm (pow2 (8 * 1) == 256);
+  assert_norm (pow2 (8 * 2) == 65536);
+  assert_norm (pow2 (8 * 3) == 16777216);
+  assert_norm (pow2 (8 * 4) == 4294967296)
+
+let parse_seq_flbytes_synth_be_int_eq
+  (len: integer_size)
+  (input: bytes)
+: Lemma
+  (
+    let _ = synth_be_int_injective len in
+    let _ = be_int_of_bounded_integer_injective len in
+    parse ((parse_seq_flbytes len `parse_synth` synth_be_int len) `parse_synth` be_int_of_bounded_integer len) input == parse (parse_bounded_integer len) input)
+=
+    let _ = synth_be_int_injective len in
+    let _ = be_int_of_bounded_integer_injective len in
+    parse_synth_eq (parse_seq_flbytes len `parse_synth` synth_be_int len) (be_int_of_bounded_integer len) input;
+    parse_synth_eq (parse_seq_flbytes len) (synth_be_int len) input
+
+
+(*
+inline_for_extraction
+let parse32_be_int_2
+: Tot (parser32 (parse_seq_flbytes 2 `parse_synth` synth_be_int len))
+= fun (input: B32.bytes) ->
+  
